@prefix war: <http://wellcomecollection.org/ontologies/article/> . 
@prefix xsd: <http://www.w3.org/2001/XMLSchema#> . 
@prefix rdf: <http://www.w3.org/1999/02/22-rdf-syntax-ns#> .
@prefix dcterms: <http://purl.org/dc/terms/> .
@prefix owl:     <http://www.w3.org/2002/07/owl#> .
@prefix rdfs:    <http://www.w3.org/2000/01/rdf-schema#> .

<http://wellcomecollection.org/ontologies/article>
    rdf:type owl:Ontology ;
    dcterms:title "Article"@en ;
    dcterms:created "2018-01-15"^^xsd:date ;
    dcterms:description "An ontology describing editorial articles and their relationships."@en .

###### classes ###  
    
war:Article rdf:type owl:Class ;
    rdfs:label "Article"@en ;
    rdfs:comment "An article"@en ;
    rdf:isDefinedBy <http://wellcomecollection.org/ontologies/article> .
    
war:ArticleType rdf:type owl:Class ;
    rdfs:label "ArticleType"@en ;
    rdfs:comment "The editoiral intent or form used by the creator. This is seperate from format. Example would be analysis or interview that could be a video or text based transcript."@en ;
    rdf:isDefinedBy <http://wellcomecollection.org/ontologies/article> .
    
war:ArticleSeries rdf:type owl:Class ;
    rdfs:label "ArticleSeries"@en ;
    rdfs:comment "A branded series of articles that can be taken together or individually."@en ;
    rdf:isDefinedBy <http://wellcomecollection.org/ontologies/article> .  

war:ArticleFormat rdf:type owl:Class ;
    rdfs:label "ArticleFormat"@en ;
    rdfs:comment "The primary format or document type of the article. For example video, text or audio."@en ;
    rdf:isDefinedBy <http://wellcomecollection.org/ontologies/article> .  

    
#### object properties ####

war:articleType rdf:type owl:ObjectProperty ;
    rdfs:label "articleType"@en ;
    rdfs:comment "Relates an article to its type."@en ;
    rdfs:domain war:Article ;
    rdfs:range war:ArticleType ;
    rdf:isDefinedBy <http://wellcomecollection.org/ontologies/article> .

war:articleFormat rdf:type owl:ObjectProperty ;
    rdfs:label "articleFormat"@en ;
    rdfs:comment "Relates an article to its format."@en ;
    rdfs:domain war:Article ;
    rdfs:range war:ArticleFormat ;
    rdf:isDefinedBy <http://wellcomecollection.org/ontologies/article> .

war:articleSeries rdf:type owl:ObjectProperty ;
    rdfs:label "articleSeries"@en ;
    rdfs:comment "Relates an article to an article series."@en ;
    rdfs:domain war:Article ;
    rdfs:range war:ArticleSeries ;
    rdf:isDefinedBy <http://wellcomecollection.org/ontologies/article> .        
    
####### data properties #####

war:positionInArticleSeries rdf:type owl:DatatypeProperty ;
    rdfs:label "positionInArticleSeries"@en ;
    rdfs:comment "The position of an article in an article series."@en ;
    rdfs:domain war:Article ;
    rdfs:range xsd:integer ; 
    rdf:isDefinedBy <http://wellcomecollection.org/ontologies/article> .
    
