@prefix wwork: <http://wellcomecollection.org/ontologies/works/> . 
@prefix xsd: <http://www.w3.org/2001/XMLSchema#> . 
@prefix rdf: <http://www.w3.org/1999/02/22-rdf-syntax-ns#> .
@prefix dcterms: <http://purl.org/dc/terms/> .
@prefix owl:     <http://www.w3.org/2002/07/owl#> .
@prefix rdfs:    <http://www.w3.org/2000/01/rdf-schema#> .

<http://wellcomecollection.org/ontologies/works>
    rdf:type owl:Ontology ;
    dcterms:title "Works ontology"@en ;
    dcterms:created "2017-02-13"^^xsd:date ;
    dcterms:description "An ontology describing library and archive works, including their physical items and relationships."@en .
    
#######  Classes #####  

wwork:Work rdf:type owl:Class ;
    rdfs:label "Work"@en ;
    rdfs:comment "An individual work such as a text, archive item or picture; or a grouping of individual works (so, for instance, an archive collection counts as a work, as do all the series and individual files within it).  Each work may exist in multiple instances (e.g. copies of the same book).  N.B. this is not synonymous with \"work\" as that is understood in the International Federation of Library Associations and Institutions' Functional Requirements for Bibliographic Records model (FRBR) but represents something lower down the FRBR hierarchy, namely manifestation. Groups of related items are also included as works because they have similar properties to the individual ones."@en ;
    rdf:isDefinedBy <http://wellcomecollection.org/ontologies/works> .
    
wwork:Item rdf:type owl:Class ;
    rdfs:label "Item"@en ;
    rdfs:comment "A specific instance of a work: for instance, an individual physical copy with its own location.  This corresponds to the bottom, Instance, layer of FRBR.  Works that are unique - that is, have only one copy - are described in terms of a Work for their intellectual content, linked to an Item describing their local (usually physical) characteristics."@en ;
    rdf:isDefinedBy <http://wellcomecollection.org/ontologies/works> .  

wwork:WorkType rdf:type owl:Class ;
    rdfs:label "WorkType"@en ;
    rdfs:comment "A broad, top-level description of the form of a work: namely, whether it is a printed book, archive, painting, photograph, moving image, etc."@en ;
    rdf:isDefinedBy <http://wellcomecollection.org/ontologies/works> .
    
wwork:Place rdf:type owl:Class ;
    rdfs:label "Place"@en ;
    rdfs:comment "A physical location that relates in some way to a work: for example, the place at which a work was published or otherwise created."@en ;
    rdf:isDefinedBy <http://wellcomecollection.org/ontologies/works> .
    
wwork:Period rdf:type owl:Class ;
    rdfs:label "Period"@en ;
    rdfs:comment "A period of time which can have a start and an end. Each of which could be reprented by a range."@en ;
    rdf:isDefinedBy <http://wellcomecollection.org/ontologies/works> .

wwork:Concept rdf:type owl:Class ;
    rdfs:label "Concept"@en ;
    rdfs:comment "A broad concept that forms part of a thesaurus-based classification of human knowledge."@en ;
    rdf:isDefinedBy <http://wellcomecollection.org/ontologies/works> .  

wwork:Genre rdf:type owl:Class ;
    rdfs:label "Genre"@en ;
    rdfs:comment "A the genre or technique of the work."@en ;
    rdf:isDefinedBy <http://wellcomecollection.org/ontologies/works> .  

wwork:Agent rdf:type owl:Class ;
    rdfs:label "Agent"@en ;
    rdfs:comment "A person, group, event or organisation."@en ;
    rdf:isDefinedBy <http://wellcomecollection.org/ontologies/works> .  
    
wwork:Language rdf:type owl:Class ;
    rdfs:label "Language"@en ;
    rdfs:comment "A language recognised as one of those in the ISO 639-2 language codes."@en ;
    rdf:isDefinedBy <http://wellcomecollection.org/ontologies/works> .  
    
wwork:Series rdf:type owl:Class ;
    rdfs:label "Series"@en ;
    rdfs:comment "A series of works."@en ;
    rdf:isDefinedBy <http://wellcomecollection.org/ontologies/works> .              
                
wwork:Subject rdf:type owl:Class ;
    rdfs:label "Subject"@en ;
    rdfs:comment "The subject of a work."@en ;
    rdf:isDefinedBy <http://wellcomecollection.org/ontologies/works> .  
    
wwork:Contributor rdf:type owl:Class ;
    rdfs:label "Contributor"@en ;
    rdfs:comment "A contribution to a work."@en ;
    rdf:isDefinedBy <http://wellcomecollection.org/ontologies/works> .      
                    
wwork:ProductionEvent rdf:type owl:Class ;
    rdfs:label "ProductionEvent"@en ;
    rdfs:comment "An event contributing to the production, publishing or distribution of a work."@en ;
    rdf:isDefinedBy <http://wellcomecollection.org/ontologies/works> . 
  
                    
#######  Object properties ##### 
    

wwork:items rdf:type owl:ObjectProperty ;
    rdfs:label "items"@en ;
    rdfs:comment "Relates the general bibliographic description of a work to specific instances of it, each item forming a unique incarnation of that work.  Item here corresponds to the bottom layer of FRBR."@en ;
    rdfs:domain wwork:Work ;
    rdfs:range wwork:Item ;
    rdf:isDefinedBy <http://wellcomecollection.org/ontologies/works> .

wwork:isPartOf rdf:type owl:ObjectProperty ;
    rdfs:label "isPartOf"@en ;
    rdfs:comment "Relates an work to its host work."@en ;
    rdfs:domain wwork:Work ;
    rdfs:range wwork:Work ;
    rdf:isDefinedBy <http://wellcomecollection.org/ontologies/works> .
    
wwork:hasPart rdf:type owl:ObjectProperty ;
    rdfs:label "hasPart"@en ;
    rdfs:comment "Relates an work to its parts."@en ;
    rdfs:domain wwork:Work ;
    rdfs:range wwork:Work ;
    rdf:isDefinedBy <http://wellcomecollection.org/ontologies/works> .    
    
wwork:isCopyOf rdf:type owl:ObjectProperty ;
    rdfs:label "isCopyOf"@en ;
    rdfs:comment "Relates an entity to one of which it forms a copy - that is, a transcription or other duplication.  (This property is used when it results in the creation of a new bibliographic entity and not simply for second instances of a particular work.) "@en ;
    rdfs:domain wwork:Work ;
    rdfs:range wwork:Work ;
    rdf:isDefinedBy <http://wellcomecollection.org/ontologies/works> .
    
wwork:isOriginalOf rdf:type owl:ObjectProperty ;
    rdfs:label "isOriginalOf"@en ;
    rdfs:comment "Relates an entity to one that forms a copy of it.  (This property is used when it results in the creation of a new bibliographic entity and not simply for second instances of a particular work.) "@en ;
    rdfs:domain wwork:Work ;
    rdfs:range wwork:Work ;
    rdf:isDefinedBy <http://wellcomecollection.org/ontologies/works> .
        
wwork:creators rdf:type owl:ObjectProperty ;
    rdfs:label "creators"@en ;
    rdfs:comment "Relates a work to its author, compiler, editor, artist or other entity responsible for its coming into existence in the form that it has."@en ;
    rdfs:domain wwork:Work ;
    rdfs:range wwork:Agent ;
    rdf:isDefinedBy <http://wellcomecollection.org/ontologies/works> .

wwork:publishers rdf:type owl:ObjectProperty ;
    rdfs:label "publishers"@en ;
    rdfs:comment "Relates a published work to its publisher."@en ;
    rdfs:domain wwork:Work ;
    rdfs:range wwork:Agent ;
    rdf:isDefinedBy <http://wellcomecollection.org/ontologies/works> .
    
wwork:placeOfPublication rdf:type owl:ObjectProperty ;
    rdfs:label "placeOfPublication"@en ;
    rdfs:comment "Relates a work to its place of publication."@en ;
    rdfs:domain wwork:Work ;
    rdfs:range wwork:Place ;
    rdf:isDefinedBy <http://wellcomecollection.org/ontologies/works> .
    
wwork:placeOfCreation rdf:type owl:ObjectProperty ;
    rdfs:label "placeOfCreation"@en ;
    rdfs:comment "Relates a work to its place of creation; typically this will be used for unpublished works, whilst published works will instead use the property hasPublicationLocation."@en ;
    rdfs:domain wwork:Work ;
    rdfs:range wwork:Place ;
    rdf:isDefinedBy <http://wellcomecollection.org/ontologies/works> .
    
wwork:subjects rdf:type owl:ObjectProperty ;
    rdfs:label "subjects"@en ;
    rdfs:comment "Relates a work to the general thesaurus-based concept that describes the work's content."@en ;
    rdfs:domain wwork:Work ;
    rdfs:range wwork:Subject ;
    rdf:isDefinedBy <http://wellcomecollection.org/ontologies/works> .

wwork:genres rdf:type owl:ObjectProperty ;
    rdfs:label "genres"@en ;
    rdfs:comment "Relates a work to its genres."@en ;
    rdfs:domain wwork:Work ;
    rdfs:range wwork:Genre ;
    rdf:isDefinedBy <http://wellcomecollection.org/ontologies/works> .
    
wwork:workType rdf:type owl:ObjectProperty ;
    rdfs:label "workType"@en ;
    rdfs:comment "Relates a Work to the general WorkType that describes the work's form: published text, painting, and so on."@en ;
    rdfs:domain wwork:Work ;
    rdfs:range wwork:WorkType ;
    rdf:isDefinedBy <http://wellcomecollection.org/ontologies/works> .
    
wwork:publicationDate rdf:type owl:DatatypeProperty ;
    rdfs:label "publicationDate"@en ;
    rdfs:comment "Relates the publication of a work to a date, when the work has been formally published.  This date is not identical with the property createdDate: for example, a work may be created at a particular time but only published after the author's death, or a work may be published in a modern edition long after first publication.  An extreme example would be the works of Aristotle, all of which are created some centuries BCE but not published in the formal sense for many centuries after this"@en ;
    rdfs:domain wwork:Work ;
    rdfs:range wwork:Period ;
    rdf:isDefinedBy <http://wellcomecollection.org/ontologies/works> .  
    
wwork:createdDate rdf:type owl:DatatypeProperty ;
    rdfs:label "createdDate"@en ;
    rdfs:comment "Relates the creation of a work to a date, when the date of creation does not cover a range"@en ;
    rdfs:domain wwork:Work ;
    rdfs:range wwork:Period ;
    rdf:isDefinedBy <http://wellcomecollection.org/ontologies/works> . 
    
wwork:language rdf:type owl:DatatypeProperty ;
    rdfs:label "language"@en ;
    rdfs:comment "Relates a work to its primary language"@en ;
    rdfs:domain wwork:Work ;
    rdfs:range wwork:Language ;
    rdf:isDefinedBy <http://wellcomecollection.org/ontologies/works> .
    
wwork:series rdf:type owl:DatatypeProperty ;
    rdfs:label "series"@en ;
    rdfs:comment "Relates a work to a series it is a part of"@en ;
    rdfs:domain wwork:Work ;
    rdfs:range wwork:Series ;
    rdf:isDefinedBy <http://wellcomecollection.org/ontologies/works> .  
    
wwork:works rdf:type owl:DatatypeProperty ;
    rdfs:label "works"@en ;
    rdfs:comment "Relates a series to works that are part of it"@en ;
    rdfs:domain wwork:Work ;
    rdfs:range wwork:Series ;
    rdf:isDefinedBy <http://wellcomecollection.org/ontologies/works> . 
    
wwork:contributors rdf:type owl:DatatypeProperty ;
    rdfs:label "contributors"@en ;
    rdfs:comment "Relates a work to contributors to that work"@en ;
    rdfs:domain wwork:Work ;
    rdfs:range wwork:Contributor ;
    rdf:isDefinedBy <http://wellcomecollection.org/ontologies/works> .  
    
wwork:agent rdf:type owl:DatatypeProperty ;
    rdfs:label "agent"@en ;
    rdfs:comment "Relates an contribution to the responsible agent."@en ;
    rdfs:domain wwork:Contributor ;
    rdfs:range wwork:Agent ;
    rdf:isDefinedBy <http://wellcomecollection.org/ontologies/works> .  
        
wwork:roles rdf:type owl:DatatypeProperty ;
    rdfs:label "roles"@en ;
    rdfs:comment "Relates a contributor to the role they played in the contribution."@en ;
    rdfs:domain wwork:Contributor ;
    rdfs:range wwork:ContributorRole ;
    rdf:isDefinedBy <http://wellcomecollection.org/ontologies/works> . 
    
wwork:classification rdf:type owl:DatatypeProperty ;
    rdfs:label "classification"@en ;
    rdfs:comment "Relates a work to its classifications."@en ;
    rdfs:domain wwork:Work ;
    rdfs:range wwork:Concept ;
    rdf:isDefinedBy <http://wellcomecollection.org/ontologies/works> . 
    
wwork:production rdf:type owl:DatatypeProperty ;
    rdfs:label "provisionEvents"@en ;
    rdfs:comment "Relates a work to its provision events."@en ;
    rdfs:domain wwork:Work ;
    rdfs:range wwork:ProductionEvent ;
    rdf:isDefinedBy <http://wellcomecollection.org/ontologies/works> . 
    
wwork:productionFunction rdf:type owl:DatatypeProperty ;
    rdfs:label "productionFunction"@en ;
    rdfs:comment "Relates a production event to a specific function."@en ;
    rdfs:domain wwork:ProductionEvent ;
    rdfs:range wwork:Concept ;
    rdf:isDefinedBy <http://wellcomecollection.org/ontologies/works> .                                              
    
#######  Data properties #####  
                        
    
wwork:modifiedDate rdf:type owl:DatatypeProperty ;
    rdfs:label "modifiedDate"@en ;
    rdfs:comment "Relates the last recorded modification of a work to a date"@en ;
    rdfs:domain wwork:Work ;
    rdfs:range xsd:dateTime ;
    rdf:isDefinedBy <http://wellcomecollection.org/ontologies/works> .  

wwork:title rdf:type owl:DatatypeProperty ;
    rdfs:label "title"@en ;
    rdfs:comment "The title or other short label of a work, including labels not present in the actual work or item but applied by the cataloguer for the purposes of search or description."@en ;
    rdfs:domain wwork:Work ;
    rdfs:range rdf:langString ; 
    rdf:isDefinedBy <http://wellcomecollection.org/ontologies/works> .  
        
wwork:partNumber rdf:type owl:DatatypeProperty ;
    rdfs:label "partNumber"@en ;
    rdfs:comment "The part number the work is in a group or series of works."@en ;
    rdfs:domain wwork:Work ;
    rdfs:range rdf:langString ; 
    rdf:isDefinedBy <http://wellcomecollection.org/ontologies/works> .  
        
wwork:partName rdf:type owl:DatatypeProperty ;
    rdfs:label "partName"@en ;
    rdfs:comment "The part name for the work in a group or series of works."@en ;
    rdfs:domain wwork:Work ;
    rdfs:range rdf:langString ; 
    rdf:isDefinedBy <http://wellcomecollection.org/ontologies/works> .  
        
wwork:level rdf:type owl:DatatypeProperty ;
    rdfs:label "level"@en ;
    rdfs:comment "Indicates the position of a work within a hierarchy of works: for example, Collection, Series, Item etc. The terminology used here will typically be drawn from external systems and may not necessarily correspond directly to the terminology of this ontology: for instance, in archive catalogues the term Item may be used to describe an entity that combines properties assigned in this ontology to the Work and Item classes."@en ;
    rdfs:domain wwork:Work ;
    rdfs:range xsd:integer ; 
    rdf:isDefinedBy <http://wellcomecollection.org/ontologies/works> .

wwork:alternativeTitle rdf:type owl:DatatypeProperty ;
    rdfs:label "alternativeTitle"@en ;
    rdfs:comment "Alternative title for a work, usually used for published material: former title, variant forms, translation of main title, etc."@en ;
    rdfs:domain wwork:Work ;
    rdfs:range rdf:langString ; 
    rdf:isDefinedBy <http://wellcomecollection.org/ontologies/works> .
        
wwork:lettering rdf:type owl:DatatypeProperty ;
    rdfs:label "lettering"@en ;
    rdfs:comment "Recording written text on a (usually visual) work."@en ;
    rdfs:domain wwork:Work ;
    rdfs:range rdf:langString ; 
    rdf:isDefinedBy <http://wellcomecollection.org/ontologies/works> .
    
wwork:physicalDescription rdf:type owl:DatatypeProperty ;
    rdfs:label "physicalDescription"@en ;
    rdfs:comment "A description of specific physical characteristics of the item - condition, dimensions, details of cover or binding, etc. - or, in the case of digital objects, any notes relating to this digital manifestation over and above notes of file format."@en ;
    rdfs:domain wwork:Work ;
    rdfs:range rdf:langString ;
    rdf:isDefinedBy <http://wellcomecollection.org/ontologies/works> .
    
wwork:extent rdf:type owl:DatatypeProperty ;
    rdfs:label "extent"@en ;
    rdfs:comment "Number of physical pages, volumes, cassettes, total playing time, etc., of of each type of unit."@en ;
    rdfs:domain wwork:Work ;
    rdfs:range rdf:langString ;
    rdf:isDefinedBy <http://wellcomecollection.org/ontologies/works> . 
    
wwork:dimensions rdf:type owl:DatatypeProperty ;
    rdfs:label "dimensions"@en ;
    rdfs:comment "Expressed in centimeters, millimeters, or inches; may include a parenthetical qualifier giving the format of the item (e.g., (fol.), (8vo))."@en ;
    rdfs:domain wwork:Work ;
    rdfs:range rdf:langString ;
    rdf:isDefinedBy <http://wellcomecollection.org/ontologies/works> .  
    
wwork:positionInSeries rdf:type owl:DatatypeProperty ;
    rdfs:label "positionInSeries"@en ;
    rdfs:comment "Position in series or volume number."@en ;
    rdfs:domain wwork:Work ;
    rdfs:range xsd:integer ;
    rdf:isDefinedBy <http://wellcomecollection.org/ontologies/works> .            
    
